src/QueryStructure/Specification/SearchTerms/ListPrefix.v
@@ -1,0 +1,54 @@
+Require Import ADTSynthesis.QueryStructure.Specification.Representation.QueryStructureNotations.
+
+Open Scope list.
+
+Section PrefixClauses.
+  Context {X : Type}
+          {X_eq_dec : Query_eq X}.
+
+  Definition IsPrefix (p s : list X) : Prop := exists e, p ++ e = s.
+
+  Fixpoint IsPrefix_dec (p s : list X) : {IsPrefix p s} + {~ IsPrefix p s}.
+  refine (match p, s with
+            | nil, _ => left _
+            | p' :: ps, s' :: ss =>
+              if A_eq_dec p' s' then
+                if IsPrefix_dec ps ss then
+                  left _
+                else
+                  right _
+              else
+                right _
+            | _, _ => right _
+          end); intuition; [
+    eexists; intuition |
+    inject H; apply app_eq_nil in H0; destruct H0; inversion H |
+    destruct _H0; eexists; simpl; subst |
+    apply _H0; inject H; inversion H0; eexists |
+    inject H; simpl in H0; inversion H0 ]; eauto.
+  Defined.
+
+  Ltac prefix_crush := intros; find_if_inside; intuition eauto; discriminate.
+
+  Instance DecideableEnsemble_HasPrefix st :
+    DecideableEnsemble (IsPrefix st) :=
+    {| dec a := ?[IsPrefix_dec st a] |}. prefix_crush. Defined.
+
+  Global Instance DecideableEnsemble_HasPrefix_f
+         (A : Type)
+         (f : A -> list X)
+         b :
+    DecideableEnsemble (fun a => IsPrefix b (f a)) :=
+    {| dec a := ?[IsPrefix_dec b (f a)] |}. prefix_crush. Defined.
+
+  Instance DecideableEnsemble_FindPrefix st :
+    DecideableEnsemble (fun a => IsPrefix a st) :=
+    {| dec a := ?[IsPrefix_dec a st] |}. prefix_crush. Defined.
+
+  Global Instance DecideableEnsemble_FindPrefix_f
+         (A : Type)
+         (f : A -> list X)
+         b :
+    DecideableEnsemble (fun a => IsPrefix (f a) b) :=
+    {| dec a := ?[IsPrefix_dec (f a) b] |}. prefix_crush. Defined.
+End PrefixClauses.
